

# Backwards Martingales and Exchangeability

김지수 (Jisu KIM)

학률론 2 (Probability Theory 2), 2025 2nd semester (fall)

Some parts of this lecture note are from the lecture notes from Prof. Alessandro Rianllo's "Advanced Probability Overview".

## Backwards Martingales

A backwards martingale (some authors call them *reversed*) is a martingale indexed by the negative integers, i.e.  $X_n$ ,  $n \leq 0$ , adapted to an increasing sequence of  $\sigma$ -fields  $\mathcal{F}_n$  with

$$\mathbb{E}[X_{n+1} | \mathcal{F}_n] = X_n, \quad n \leq -1.$$

Because the  $\sigma$ -fields decrease as  $n \downarrow -\infty$ , the convergence theory for backwards martingales is particularly simple.

**Theorem** ([2, Theorem 4.7.1]).  $X_{-\infty} = \lim_{n \rightarrow -\infty} X_n$  exists a.s. and in  $L^1$ .

*Proof.* Let  $U_n$  be the number of upcrossings of  $[a, b]$  by  $X_{-n}, \dots, X_0$ . The upcrossing inequality [2, Theorem 4.2.10] implies

$$(b - a)\mathbb{E}U_n \leq \mathbb{E}(X_0 - a)^+.$$

Letting  $n \rightarrow \infty$  and using the monotone convergence theorem, we have  $\mathbb{E}U_\infty < \infty$ , so by the remark after [2, Theorem 4.2.11], the limit  $X_{-\infty}$  exists a.s.. The martingale property implies  $X_n = \mathbb{E}[X_0 | \mathcal{F}_n]$ , so [2, Theorem 4.6.1] implies  $X_n$  is uniformly integrable and [2, Theorem 4.6.3] tells us that the convergence occurs in  $L^1$ .  $\square$

The next result identifies the limit in [2, Theorem 4.7.1].

**Theorem** ([2, Theorem 4.7.2]). If  $X_{-\infty} = \lim_{n \rightarrow -\infty} X_n$  and  $\mathcal{F}_{-\infty} = \bigcap_n \mathcal{F}_n$ , then

$$X_{-\infty} = \mathbb{E}[X_0 | \mathcal{F}_{-\infty}].$$

*Proof.* Clearly  $X_{-\infty} \in \mathcal{F}_{-\infty}$ . Since  $X_n = \mathbb{E}[X_0 | \mathcal{F}_n]$ , for  $A \in \mathcal{F}_{-\infty} \subset \mathcal{F}_n$ ,

$$\int_A X_n dP = \int_A X_0 dP.$$

[2, Theorem 4.7.1] and [2, Lemma 4.6.5] imply  $\mathbb{E}[X_n; A] \rightarrow \mathbb{E}[X_{-\infty}; A]$ , so

$$\int_A X_{-\infty} dP = \int_A X_0 dP,$$

for all  $A \in \mathcal{F}_{-\infty}$ , proving the claim.  $\square$

The next result is [2, Theorem 4.6.8] backwards

**Theorem** ([2, Theorem 4.7.3]). If  $\mathcal{F}_n \downarrow \mathcal{F}_{-\infty}$  as  $n \downarrow -\infty$  (i.e.  $\mathcal{F}_{-\infty} = \bigcap_n \mathcal{F}_n$ ), then

$$\mathbb{E}[Y \mid \mathcal{F}_n] \rightarrow \mathbb{E}[Y \mid \mathcal{F}_{-\infty}] \quad \text{a.s. and in } L^1.$$

*Proof.*  $X_n = \mathbb{E}[Y \mid \mathcal{F}_n]$  is a backwards martingale, so [2, Theorem 4.7.1]-[2, Theorem 4.7.2] imply that as  $n \downarrow -\infty$ ,  $X_n \rightarrow X_{-\infty}$  a.s. and in  $L^1$ , where

$$X_{-\infty} = \mathbb{E}[X_0 \mid \mathcal{F}_{-\infty}] = \mathbb{E}[\mathbb{E}[Y \mid \mathcal{F}_0] \mid \mathcal{F}_{-\infty}] = \mathbb{E}[Y \mid \mathcal{F}_{-\infty}].$$

□

## Exchangeability

Even though the convergence theory for backwards martingales is easy, there are some nice applications, in particular for exchangeable random variables.

**Definition.** A sequence of random quantities  $\{X_n\}_{n=1}^\infty$  is *exchangeable* if, for every  $n$  and all distinct  $j_1, \dots, j_n$ ,  $(X_{j_1}, \dots, X_{j_n})$  and  $(X_1, \dots, X_n)$  have the same joint distribution.

*Remark* ([2, Example 4.7.8]). This definition is equivalent to that, for every  $n$  and any permutation  $\pi$  of  $\{1, \dots, n\}$ ,  $(X_1, \dots, X_n)$  and  $(X_{\pi(1)}, \dots, X_{\pi(n)})$  have the same joint distribution.

**Example** (Conditionally iid random quantities). Let  $\{X_n\}_{n=1}^\infty$  be conditionally iid given a  $\sigma$ -field  $\mathcal{F}$ . Then  $\{X_n\}_{n=1}^\infty$  is an exchangeable sequence. The result follows easily from the fact that

$$\mu_{X_{j_1}, \dots, X_{j_n} \mid \mathcal{F}} = \mu_{X_1, \dots, X_n \mid \mathcal{F}} \quad \text{a.s.}$$

To analyze an exchangeable sequence of random variables, we return to the special space utilized for Hewitt-Savage 0-1 law in Section 2.5. That is, we suppose

$$\Omega = \{(\omega_1, \omega_2, \dots) : \omega_i \in S\}, \quad \mathcal{F} = S \times S \times \dots, \quad X_n(\omega) = \omega_n.$$

Let  $\mathcal{E}_n$  be the  $\sigma$ -field generated by events that are invariant under permutations leaving  $n+1, n+2, \dots$  fixed, and let  $\mathcal{E} = \bigcap_n \mathcal{E}_n$  be the exchangeable  $\sigma$ -field.

We recall Hewitt-Savage 0-1 law, which is a generalization of Kolmogorov's 0-1 law. We provide martingale proof of this at Appendix.

**Theorem** ([2, Theorem 2.5.4, Example 4.7.6]). *Hewitt-Savage 0-1 law.* If  $X_1, X_2, \dots$  are i.i.d. and  $A \in \mathcal{E}$  then  $P(A) \in \{0, 1\}$ .

**Theorem.** *Strong Law of Large Numbers.* Let  $\{X_n\}_{n=1}^\infty$  be an exchangeable sequence of random variables with  $\mathbb{E}|X_i| < \infty$ . Let  $S_n = \xi_1 + \dots + \xi_n$ . Then  $\lim_{n \rightarrow \infty} S_n/n$  exists a.s. and has mean equal to  $\mathbb{E}[X_1]$ . If the  $X_j$ 's are independent, then the limit equals  $\mathbb{E}[X_1]$  a.s.

*Proof.* Let  $Y_{-n} = S_n/n$ , and let  $\{\mathcal{F}_{-n}\}_{n \geq 0}$  be defined as

$$\mathcal{F}_{-n} = \sigma(S_n, S_{n+1}, S_{n+2}, \dots) = \sigma(S_n, X_{n+1}, X_{n+2}, \dots).$$

To compute  $\mathbb{E}[Y_{-n} \mid \mathcal{F}_{-n-1}]$ , note that if  $j, k \leq n+1$ , symmetry (specifically, HW#1 Problem 7) implies  $\mathbb{E}[X_j \mid$

$\mathcal{F}_{-n-1}] = \mathbb{E}[X_k \mid \mathcal{F}_{-n-1}]$ , so

$$\mathbb{E}[X_{n+1} \mid \mathcal{F}_{-n-1}] = \frac{1}{n+1} \sum_{k=1}^{n+1} \mathbb{E}[X_k \mid \mathcal{F}_{-n-1}] = \frac{1}{n+1} \mathbb{E}[S_{n+1} \mid \mathcal{F}_{-n-1}] = \frac{S_{n+1}}{n+1}.$$

Since  $Y_{-n} = (S_{n+1} - X_{n+1})/n$ , it follows that

$$\mathbb{E}[Y_{-n} \mid \mathcal{F}_{-n-1}] = \mathbb{E}[S_{n+1}/n \mid \mathcal{F}_{-n-1}] - \mathbb{E}[X_{n+1}/n \mid \mathcal{F}_{-n-1}] = \frac{S_{n+1}}{n+1} = Y_{-n-1}.$$

Thus  $Y_{-n}$  is a backwards martingale adapted to  $\{\mathcal{F}_{-n}\}_{n \geq 0}$ , so by [2, Theorem 4.7.1]-[2, Theorem 4.7.2],

$$\lim_{n \rightarrow \infty} Y_{-n} = \lim_{n \rightarrow \infty} S_n/n = \mathbb{E}[Y_{-1} \mid \mathcal{F}_{-\infty}] = \mathbb{E}[X_1 \mid \mathcal{F}_{-\infty}].$$

In particular,

$$\mathbb{E} \left[ \lim_{n \rightarrow \infty} Y_{-n} \right] = \mathbb{E} [\mathbb{E}[X_1 \mid \mathcal{F}_{-\infty}]] = \mathbb{E}[X_1].$$

Suppose further that  $X_j$ 's are independent. Since  $\mathcal{F}_{-n} \subset \mathcal{E}_n$ ,  $\mathcal{F}_{-\infty} \subset \mathcal{E}$ . The Hewitt–Savage 0–1 law [2, Theorem 2.5.4, Example 4.7.6] says  $\mathcal{E}$  is trivial, so

$$\lim_{n \rightarrow \infty} S_n/n = \mathbb{E}[X_{-1}] \quad \text{a.s.}$$

□

**Example.** Let  $\{X_n\}_{n=1}^{\infty}$  be Bernoulli random variables such that

$$P(X_1 = x_1, \dots, X_n = x_n) = \frac{1}{(n+1) \binom{n}{y}},$$

where  $y = \sum_{j=1}^n x_j$ . One can show that this specifies consistent joint distributions. One can also check that the  $X_n$ 's are not independent:

$$P(X_1 = 1) = \frac{1}{2}, \quad P(X_1 = 1, X_2 = 1) = \frac{1}{3} \neq \left(\frac{1}{2}\right)^2.$$

From Strong law of large number, we know that  $Y_{-n} := S_n/n$  converges a.s., hence it converges in distribution. We can compute the exact distribution:

$$P(Y_{-n} = k/n) = \frac{1}{n+1}, \quad k = 0, 1, \dots, n.$$

Hence  $Y_{-n}$  converges in distribution to Uniform[0, 1], which must be the distribution of the limit. The limit is not a.s. constant.

De Finetti's theorem says that a sequence of random quantities is exchangeable if and only if it is conditionally iid given exchangeable  $\sigma$ -field. That is, the Conditionally iid example is essentially the only example of exchangeable sequences. We provide the proof at Appendix.

**Theorem** ([2, Theorem 4.7.9]). *de Finetti's Theorem.*  $X_1, X_2, \dots$  are exchangeable if and only if, conditional on  $\mathcal{E}$ ,  $X_1, X_2, \dots$  are independent and identically distributed.

When the  $X_i$  take values in a nice space, there is a regular conditional distribution for  $(X_1, X_2, \dots)$  given  $\mathcal{E}$ , and the sequence can be represented as a mixture of i.i.d. sequences. [4] call the sequence *presentable* in this case. For general measurable spaces the result may fail; see [1] and [3] for counterexamples.

## References

- [1] Lester E. Dubins and David A. Freedman. Exchangeable processes need not be mixtures of independent, identically distributed random variables. *Zeitschrift für Wahrscheinlichkeitstheorie und Verwandte Gebiete*, 1979.
- [2] Rick Durrett. *Probability—theory and examples*, volume 49 of *Cambridge Series in Statistical and Probabilistic Mathematics*. Cambridge University Press, Cambridge, 2019. Fifth edition.
- [3] David A. Freedman. A mixture of independent identically distributed random variables need not admit a regular conditional probability given the exchangeable  $\sigma$ -field. *Zeitschrift für Wahrscheinlichkeitstheorie und Verwandte Gebiete*, 1980.
- [4] Edwin Hewitt and Leonard J. Savage. Symmetric measures on Cartesian products. *Trans. Amer. Math. Soc.*, 80:470–501, 1955.

## Appendix

The key to the martingale proof for Hewitt-Savage 0-1 law and de Finetti’s Theorem is:

**Lemma** ([2, Lemma 4.7.7]). *Suppose  $X_1, X_2, \dots$  are i.i.d. and let*

$$A_n(\varphi) = \frac{1}{(n)_k} \sum_i \varphi(X_{i_1}, \dots, X_{i_k}),$$

*where the sum is over all sequences of distinct integers  $1 \leq i_1, \dots, i_k \leq n$ , and*

$$(n)_k = n(n-1) \cdots (n-k+1)$$

*is the number of such sequences. If  $\varphi$  is bounded,  $A_n(\varphi) \rightarrow \mathbb{E}\varphi(X_1, \dots, X_k)$  a.s..*

*Proof.*  $A_n(\varphi) \in \mathcal{E}_n$ , so

$$A_n(\varphi) = \mathbb{E}(A_n(\varphi) \mid \mathcal{E}_n) = \frac{1}{(n)_k} \sum_i \mathbb{E}(\varphi(X_{i_1}, \dots, X_{i_k}) \mid \mathcal{E}_n) = \mathbb{E}(\varphi(X_1, \dots, X_k) \mid \mathcal{E}_n),$$

since all the terms in the sum are the same. [2, Theorem 4.7.3] with  $\mathcal{F}_{-m} = \mathcal{E}_m$  for  $m \geq 1$  implies that

$$\mathbb{E}(\varphi(X_1, \dots, X_k) \mid \mathcal{E}_n) \rightarrow \mathbb{E}(\varphi(X_1, \dots, X_k) \mid \mathcal{E}).$$

We want to show that the limit is  $\mathbb{E}(\varphi(X_1, \dots, X_k))$ . The first step is to observe that there are  $k(n-1)^{k-1}$  terms in  $A_n(\varphi)$  involving  $X_1$ , and  $\varphi$  is bounded, so if we let  $1 \in i$  denote the sum over sequences that contain 1,

$$\frac{1}{(n)_k} \sum_{1 \in i} \varphi(X_{i_1}, \dots, X_{i_k}) \leq \frac{k(n-1)^{k-1}}{(n)_k} \sup \varphi \rightarrow 0.$$

This shows that  $\mathbb{E}(\varphi(X_1, \dots, X_k) \mid \mathcal{E}) \in \sigma(X_2, X_3, \dots)$ . Repeating the argument for  $2, 3, \dots, k$  shows

$$\mathbb{E}(\varphi(X_1, \dots, X_k) \mid \mathcal{E}) \in \sigma(X_{k+1}, X_{k+2}, \dots).$$

Intuitively, if the conditional expectation of a r.v. is independent of the r.v., then

$$\mathbb{E}(\varphi(X_1, \dots, X_k) \mid \mathcal{E}) = \mathbb{E}(\varphi(X_1, \dots, X_k)). \quad (1)$$

To show this, we prove:

$$\text{If } \mathbb{E}X^2 < \infty \text{ and } \mathbb{E}(X \mid \mathcal{G}) \in \mathcal{F} \text{ with } X \text{ independent of } \mathcal{F}, \text{ then } \mathbb{E}(X \mid \mathcal{G}) = \mathbb{E}X. \quad (2)$$

To prove (2), let  $Y = \mathbb{E}(X \mid \mathcal{G})$  and note that [2, Theorem 4.1.11] implies  $\mathbb{E}Y^2 \leq \mathbb{E}X^2 < \infty$ . By independence,  $\mathbb{E}XY = \mathbb{E}X\mathbb{E}Y = (\mathbb{E}Y)^2$  since  $\mathbb{E}Y = \mathbb{E}X$ . From the geometric interpretation of conditional expectation [2, Theorem 4.1.15],  $\mathbb{E}((X - Y)Y) = 0$ , so  $\mathbb{E}Y^2 = \mathbb{E}XY = (\mathbb{E}Y)^2$  and hence  $\text{var}(Y) = 0$ .  $\square$

Now we use this Lemma to show Hewitt-Savage 0-1 law.

*Proof.* Statement (1) holds for all bounded  $\varphi$ , so  $\mathcal{E}$  is independent of  $\mathcal{G}_k = \sigma(X_1, \dots, X_k)$ . Since this holds for all  $k$ , and  $\bigcup_k \mathcal{G}_k$  is a  $\pi$ -system containing  $\Omega$ , [2, Theorem 2.1.6] implies  $\mathcal{E}$  is independent of  $\sigma(\bigcup_k \mathcal{G}_k) \supset \mathcal{E}$ , and we get the usual 0-1 law conclusion: if  $A \in \mathcal{E}$ , it is independent of itself, and hence

$$P(A) = P(A \cap A) = P(A)P(A),$$

i.e.  $P(A) \in \{0, 1\}$ .  $\square$

We also use this Lemma to show de Finetti's Theorem.

*Proof.* Repeating the first calculation in [2, Lemma 4.7.7] and using the notation introduced there shows that for any exchangeable sequence:

$$A_n(\varphi) = \mathbb{E}(A_n(\varphi) \mid \mathcal{E}_n) = \frac{1}{(n)_k} \sum_i \mathbb{E}(\varphi(X_{i_1}, \dots, X_{i_k}) \mid \mathcal{E}_n) = \mathbb{E}(\varphi(X_1, \dots, X_k) \mid \mathcal{E}_n),$$

since all terms are the same. Again, [2, Theorem 4.7.3] implies that

$$A_n(\varphi) \rightarrow \mathbb{E}(\varphi(X_1, \dots, X_k) \mid \mathcal{E}). \quad (3)$$

This time, however,  $\mathcal{E}$  may be nontrivial, so we cannot hope that the limit is  $\mathbb{E}(\varphi(X_1, \dots, X_k))$ .

Let  $f$  and  $g$  be bounded functions on  $\mathbb{R}^{k-1}$  and  $\mathbb{R}$ , respectively. If we let  $I_{n,k}$  be the set of all sequences of distinct integers  $1 \leq i_1, \dots, i_k \leq n$ , then

$$\begin{aligned} (n)_{k-1} A_n(f) n A_n(g) &= \sum_{i \in I_{n,k-1}} f(X_{i_1}, \dots, X_{i_{k-1}}) \sum_m g(X_m) \\ &= \sum_{i \in I_{n,k}} f(X_{i_1}, \dots, X_{i_{k-1}}) g(X_{i_k}) + \sum_{i \in I_{n,k-1}} \sum_{j=1}^{k-1} f(X_{i_1}, \dots, X_{i_{k-1}}) g(X_{i_j}). \end{aligned}$$

If we let  $\varphi(x_1, \dots, x_k) = f(x_1, \dots, x_{k-1})g(x_k)$ , note that

$$\frac{(n)_{k-1}n}{(n)_k} = \frac{n}{n-k+1}, \quad \frac{(n)_{k-1}}{(n)_k} = \frac{1}{n-k+1},$$

then rearrange to get

$$A_n(\varphi) = \frac{n}{n-k+1} A_n(f) A_n(g) - \frac{1}{n-k+1} \sum_{j=1}^{k-1} A_n(\varphi_j),$$

where  $\varphi_j(x_1, \dots, x_{k-1}) = f(x_1, \dots, x_{k-1})g(x_j)$ . Applying (3) to  $\varphi$ ,  $f$ ,  $g$ , and all  $\varphi_j$  gives

$$\mathbb{E}(f(X_1, \dots, X_{k-1})g(X_k) \mid \mathcal{E}) = \mathbb{E}(f(X_1, \dots, X_{k-1}) \mid \mathcal{E})\mathbb{E}(g(X_k) \mid \mathcal{E}).$$

It follows by induction that

$$\mathbb{E} \left( \prod_{j=1}^k f_j(X_j) \middle| \mathcal{E} \right) = \prod_{j=1}^k \mathbb{E}(f_j(X_j) \mid \mathcal{E}).$$

□